src/tls/Extracted.mk
@@ -1,0 +1,154 @@
+include Makefile
+
+mlclean:
+	$(MAKE) -C $(FSTAR_HOME)/ulib/ml clean MEM=HST
+	$(MAKE) -C $(FSTAR_HOME)/ucontrib/CoreCrypto/ml clean
+	$(MAKE) -C $(FSTAR_HOME)/ucontrib/Platform/ml clean
+	$(MAKE) -C $(HACL_HOME)/secure_api/LowCProvider clean
+	$(MAKE) -C $(FFI_HOME) clean
+	-rm -rf test/*.cm* test/*.o
+	-rm -fr $(ODIR)/*.cm* $(ODIR)/*.o $(ODIR)/.deporder *.exe *.cm* *.o *.so *.dll *.out
+
+.PHONY: mlclean
+
+# Makefile voodoo to substitute _ for . in module names
+# Note that this is not sound if the F* module name contains an underscore (e.g. AEAD_GCM.fst)
+# The dependencies are handled by the .depend files above to allow semi-incremental extraction
+# (it is only incremental on connected components of the dependency graph rather than on a per-module basis)
+.SECONDEXPANSION:
+$(ODIR)/%.ml: $$(subst _,.,%.fst)
+	$(FSTAR) $(FSTAR_INCLUDE_PATHS) --lax --codegen OCaml \
+	--odir $(ODIR) $(NOEXTRACT) \
+	$(addprefix --codegen-lib , $(CODEGEN_LIBS)) \
+	--include concrete-flags $<
+
+$(ODIR)/Test%.ml: test/Test%.fst
+	$(FSTAR) $(FSTAR_INCLUDE_PATHS) --lax --codegen OCaml \
+	--odir $(ODIR) $(NOEXTRACT) \
+	$(addprefix --codegen-lib , $(CODEGEN_LIBS)) \
+	--include concrete-flags --extract_module Test$(*F) $<
+
+# Special case for Crypto.AEAD.*: must look in hacl-star/secure_api/aead
+# Note that dependencies have absolute paths in the .depend so there is no need 
+# to specialize for other internal Hacl paths
+$(ODIR)/Crypto_AEAD_%.ml: $(LLDIR)/aead/Crypto.AEAD.%.fst
+	$(FSTAR) $(FSTAR_INCLUDE_PATHS) --lax --codegen OCaml \
+	--odir $(ODIR) $(NOEXTRACT) \
+	$(addprefix --codegen-lib , $(CODEGEN_LIBS)) \
+	--include concrete-flags $<
+
+# Hacl flags: extract with concrete
+$(ODIR)/Flag.ml: $(LLDIR)/test/Flag.fst
+	$(FSTAR) $(FSTAR_INCLUDE_PATHS) --lax --codegen OCaml \
+	--odir $(ODIR) $(NOEXTRACT) \
+	$(addprefix --codegen-lib , $(CODEGEN_LIBS)) \
+	--include concrete-flags $<
+
+# Try to only rebuild fstarlib when necessary
+$(FSTAR_HOME)/ulib/ml/fstarlib.cmxa: \
+       		$(wildcard $(FSTAR_HOME)/ulib/*.fst) \
+		$(wildcard $(FSTAR_HOME)/ulib/ml/*.ml) \
+	       	$(wildcard $(FSTAR_HOME)/ulib/ml/extracted/*.ml) \
+		$(wildcard $(FSTAR_HOME)/ulib/ml/hyperstack/*.ml)
+	make -C $(FSTAR_HOME)/ulib/ml MEM=HST
+
+# Try to only rebuild CoreCrypto when necessary
+$(FSTAR_HOME)/ucontrib/CoreCrypto/ml/CoreCrypto.cmi $(FSTAR_HOME)/ucontrib/CoreCrypto/ml/CoreCrypto.cmx $(FSTAR_HOME)/ucontrib/CoreCrypto/ml/CoreCrypto.cmxa: \
+		$(FSTAR_HOME)/ucontrib/CoreCrypto/ml/CoreCrypto.ml
+	make -C $(FSTAR_HOME)/ucontrib/CoreCrypto/ml
+
+# Try to only rebuild LowCProvider when necessary
+# Missing: not dependency on hacl-star/code/*
+$(LCDIR)/LowCProvider.cmxa: $(FSTAR_HOME)/ucontrib/CoreCrypto/ml/CoreCrypto.cmxa $(wildcard $(LLDIR)/*/*.fst)
+	make -C $(LCDIR)
+
+$(FFI_HOME)/FFICallbacks.cmxa: $(wildcard $(FFI_HOME)/*.ml) $(wildcard $(FFI_HOME)/*.c)
+	make -C $(FFI_HOME)
+
+%.cmi %.cmx: %.ml
+	ocamlfind ocamlopt $(OCAMLOPTS) $(OCAML_INCLUDE_PATHS) -c $<
+
+.depend-ML: \
+	$(ODIR)/Flag.ml \
+	$(ODIR)/CommonDH.ml \
+	$(ODIR)/Crypto_AEAD_Main.ml \
+	$(ODIR)/HandshakeLog.ml \
+	$(ODIR)/Handshake.ml \
+	$(ODIR)/FFI.ml \
+	$(ODIR)/TestAPI.ml \
+	$(ODIR)/TestFFI.ml
+	ocamlfind ocamldep -native -slash -all $(OCAMLPKG) $(OCAML_INCLUDE_PATHS) $(addsuffix /*.ml,$(OCAML_PATHS)) > .depend-ML
+
+-include .depend-ML
+
+$(ODIR)/.deporder: $(ODIR)/FFI.cmx $(ODIR)/TestAPI.cmx $(ODIR)/TestFFI.cmx
+	echo `ls -rt output/*.cmx` > $(ODIR)/.deporder
+
+mitls.cmxa: \
+	$(FSTAR_HOME)/ulib/ml/fstarlib.cmxa \
+       	$(FSTAR_HOME)/ucontrib/CoreCrypto/ml/CoreCrypto.cmxa \
+       	$(LCDIR)/LowCProvider.cmxa \
+	$(FFI_HOME)/FFICallbacks.cmxa \
+	$(ODIR)/.deporder $(ODIR)/FFI.cmx
+	ocamlfind ocamlopt $(OCAML_INCLUDE_PATHS) -a `cat $(ODIR)/.deporder` -o mitls.cmxa
+
+mitls.exe: mitls.cmxa test/mitls.cmx
+	ocamlfind ocamlopt $(OCAMLOPTS) $(OCAML_INCLUDE_PATHS) -I test/ -g \
+	$(FSTAR_HOME)/ulib/ml/fstarlib.cmxa \
+	$(FSTAR_HOME)/ucontrib/CoreCrypto/ml/CoreCrypto.cmxa \
+	$(LCDIR)/lowc_stub.o $(LCDIR)/libllcrypto.a $(LCDIR)/LowCProvider.cmx \
+	$(FFI_HOME)/FFICallbacks.cmxa \
+	mitls.cmxa test/mitls.cmx -o mitls.exe
+
+test.out: mitls.cmxa $(ODIR)/TestKS.ml $(ODIR)/TestDH.ml $(ODIR)/TestGCM.ml test/parsing_test.ml test/test_hkdf.ml test/test_main.ml
+	ocamlfind ocamlopt $(OCAMLOPTS) $(OCAML_INCLUDE_PATHS) \
+	$(FSTAR_HOME)/ulib/ml/fstarlib.cmxa \
+	$(FSTAR_HOME)/ucontrib/CoreCrypto/ml/CoreCrypto.cmxa \
+	$(LCDIR)/lowc_stub.o $(LCDIR)/libllcrypto.a $(LCDIR)/LowCProvider.cmx \
+	mitls.cmxa \
+	$(ODIR)/TestKS.ml $(ODIR)/TestDH.ml $(ODIR)/TestGCM.ml test/parsing_test.ml test/test_hkdf.ml test/test_main.ml -o test.out
+
+test: test.out mitls.exe
+	# Unit tests from test/test_main.ml
+	$(EXTRA_PATH) ./test.out
+	# Run mitls.exe 
+	./mitls.exe  -v 1.2 -ffi www.google.com
+	./mitls.exe  -v 1.2 -noems www.microsoft.com
+	#./mitls.exe -v 1.3. www.google.com failing due to different draft versions
+
+# FFI support - calling from C into miTLS. TODO: remove duplication somehow
+ifeq ($(OS),Windows_NT)
+tls-ffi: mitls.cmxa
+	$(OCAML) $(OCAMLOPTS) $(OCAML_INCLUDE_PATHS) $(LIB_ML) -linkall -output-obj -g mitls.cmxa -o libmitls.dll
+else
+UNAME_S = $(shell uname -s)
+ifeq ($(UNAME_S),Darwin)
+tls-ffi: mitls.cmxa
+	$(OCAML) $(OCAMLOPTS) $(OCAML_INCLUDE_PATHS) $(LIB_ML) -linkall -runtime-variant _pic -ccopt -dynamiclib -ccopt -lasmrun -g mitls.cmxa -o libmitls.dylib
+	$(OCAML) $(OCAMLOPTS) $(OCAML_INCLUDE_PATHS) $(LIB_ML) -linkall -runtime-variant _pic -output-obj -ccopt -bundle -g mitls.cmxa -o libmitls.so
+else
+tls-ffi: mitls.cmxa
+	$(OCAML) $(OCAMLOPTS) $(OCAML_INCLUDE_PATHS) $(LIB_ML) -linkall -runtime-variant _pic -output-obj -g mitls.cmxa -o libmitls.so
+endif
+endif
+
+# our interactive tests; the baseline is make client{|12|13} vs make server 
+
+server::
+	OCAMLRUNPARAM=b ./mitls.exe -mv 1.2 -v 1.3 -s -cert ../../data/server.crt -key ../../data/server.key 127.0.0.1 4443 
+server12::
+	OCAMLRUNPARAM=b ./mitls.exe -mv 1.2 -v 1.2 -s -cert ../../data/server.crt -key ../../data/server.key 127.0.0.1 4443 
+server13::
+	OCAMLRUNPARAM=b ./mitls.exe -mv 1.3 -v 1.3 -s -cert ../../data/server.crt -key ../../data/server.key 127.0.0.1 4443 
+
+client13::
+	OCAMLRUNPARAM=b ./mitls.exe -mv 1.3 -v 1.3 127.0.0.1 4443 
+client12::
+	OCAMLRUNPARAM=b ./mitls.exe -mv 1.2 -v 1.2 127.0.0.1 4443 
+client::
+	OCAMLRUNPARAM=b ./mitls.exe -mv 1.2 -v 1.3 127.0.0.1 4443
+
+.PHONY: test tls-ffi server server12 server13 client client12 client13
+
+.DEFAULT:
+
